refinedVST/typing/int.v
@@ -495,10 +495,11 @@ Section programs.
              destruct (_ && _) eqn: Hm.
              { repeat (if_tac in Hm; try done).
                apply unsigned_eq_eq in H1; apply unsigned_eq_eq in H0; subst.
-               inv Hin.
-               ** rewrite Int.signed_mone Int.signed_repr in H1; rep_lia.
+               destruct s.
+               ** inv Hv1. contradict Hin. rewrite Int.signed_mone Int.signed_repr; rep_lia.
                ** rewrite Int.unsigned_mone in Hv2; if_tac in Hv2; inv Hv2.
-                  lapply (bitsize_small i); last by intros ->. intros; rep_lia. }
+                lapply (bitsize_small i); last by intros ->. intros; rep_lia.
+                }
              destruct s.
              ++ inv Hv1; done.
              ++ if_tac in Hv1; inv Hv1; if_tac in Hv2; inv Hv2.
@@ -512,8 +513,7 @@ Section programs.
              destruct (_ && _) eqn: Hm.
              { repeat (if_tac in Hm; try done).
                apply unsigned_inj_64 in H1; apply unsigned_inj_64 in H0; subst.
-               inv Hin.
-               rewrite Int64.signed_mone Int64.signed_repr in H1; rep_lia. }
+               inv Hin. }
              done.
           -- rewrite /Int64.eq; if_tac.
              { apply unsigned_inj_64 in H; subst; rewrite Int64.unsigned_zero in Hsc; tauto. }
@@ -532,8 +532,8 @@ Section programs.
              destruct (_ && _) eqn: Hm.
              { repeat (if_tac in Hm; try done).
                apply unsigned_eq_eq in H1; apply unsigned_eq_eq in H0; subst.
-               inv Hin.
-               ** rewrite Int.signed_mone Int.signed_repr in Hsc; rep_lia.
+               destruct s.
+               ** inv Hv1. rewrite Int.signed_mone Int.signed_repr in Hsc; rep_lia.
                ** rewrite Int.unsigned_mone in Hv2; if_tac in Hv2; inv Hv2.
                   lapply (bitsize_small i); last by intros ->. intros; rep_lia. }
              destruct s.
@@ -733,7 +733,7 @@ Section programs.
         destruct v; inv Hv.
         rewrite -Int64.neg_repr Int64.repr_signed //.
     - iApply "HΦ"; last done. iPureIntro. rewrite i2v_to_Z //.
-      inv Hin; constructor; simpl in *; rep_lia.
+      destruct it; try done; destruct s; simpl in *; try rep_lia.
   Qed.
   Definition type_neg_int_inst := [instance type_neg_int].
   Global Existing Instance type_neg_int_inst.
@@ -980,7 +980,6 @@ Section tests.
     iApply type_bin_op.
     iApply type_const_size_t. iApply type_val_int. iSplit => //.
     iApply type_const_size_t. iApply type_val_int. iSplit => //.
-    { iPureIntro. rewrite /size_t; simple_if_tac; constructor; simpl; rep_lia. }
     iApply type_arithop_int_int => //. iIntros (??). iSplit. {
       iPureIntro. (*unfold int_arithop_sidecond, elem_of, int_elem_of_it, min_int, max_int in *; lia.*) rewrite Z.add_0_r //.
     }
